theorems: implement `apply_rewrite` and `apply_rw` tactics

theorems/iN/iN_llvm.lean
@@ -1,13 +1,12 @@
 import theorems.iN.SimpSets
 import theorems.iN.iN_def
-import theorems.Core.Attrs.Attrs
 
 namespace iN
 
 @[simp_iN]
 def add? {n} (a b : BitVec n) : iN n := bitvec (a + b)
 
-@[simp_iN, inst "add"]
+@[simp_iN]
 def add {n} (x y : iN n) : iN n := pBind₂ x y add?
 
 @[simp_iN]
@@ -17,7 +16,7 @@ def addNsw? {n} (a b : BitVec n) : iN n :=
   else
     add? a b
 
-@[simp_iN, inst "add.nsw"]
+@[simp_iN]
 def addNsw {n} (x y : iN n) : iN n := pBind₂ x y addNsw?
 
 @[simp_iN]
@@ -27,7 +26,7 @@ def addNuw? {n} (a b : BitVec n) : iN n :=
   else
     add? a b
 
-@[simp_iN, inst "add.nuw"]
+@[simp_iN]
 def addNuw {n} (x y : iN n) : iN n := pBind₂ x y addNuw?
 
 @[simp_iN]
@@ -39,7 +38,7 @@ def addNw? {n} (a b : BitVec n) : iN n :=
   else
     add? a b
 
-@[simp_iN, inst "add.nw"]
+@[simp_iN]
 def addNw {n} (x y : iN n) : iN n := pBind₂ x y addNw?
 
 instance : Add (iN n) where
@@ -52,7 +51,7 @@ infixl:65 " +nw "  => iN.addNw
 @[simp_iN]
 def sub? {n} (a b : BitVec n) : iN n := bitvec (a - b)
 
-@[simp_iN, inst "sub"]
+@[simp_iN]
 def sub {n} (x y : iN n) : iN n := pBind₂ x y sub?
 
 @[simp_iN]
@@ -62,7 +61,7 @@ def subNsw? {n} (a b : BitVec n) : iN n :=
   else
     sub? a b
 
-@[simp_iN, inst "sub.nsw"]
+@[simp_iN]
 def subNsw {n} (x y : iN n) : iN n := pBind₂ x y subNsw?
 
 @[simp_iN]
@@ -72,7 +71,7 @@ def subNuw? {n} (a b : BitVec n) : iN n :=
   else
     sub? a b
 
-@[simp_iN, inst "sub.nuw"]
+@[simp_iN]
 def subNuw {n} (x y : iN n) : iN n := pBind₂ x y subNuw?
 
 @[simp_iN]
@@ -84,7 +83,7 @@ def subNw? {n} (a b : BitVec n) : iN n :=
   else
     sub? a b
 
-@[simp_iN, inst "sub.nw"]
+@[simp_iN]
 def subNw {n} (x y : iN n) : iN n := pBind₂ x y subNw?
 
 instance : Sub (iN n) where
@@ -97,61 +96,61 @@ infixl:65 " -nw "  => iN.subNw
 @[simp_iN]
 def icmpEq? {n} (x y : BitVec n) : iN 1 := bitvec (if x == y then 1 else 0)
 
-@[simp_iN, inst "icmp.eq"]
+@[simp_iN]
 def icmpEq {n} (x y : iN n) : iN 1 := pBind₂ x y icmpEq?
 
 @[simp_iN]
 def icmpNe? {n} (x y : BitVec n) : iN 1 := bitvec (if x != y then 1 else 0)
 
-@[simp_iN, inst "icmp.ne"]
+@[simp_iN]
 def icmpNe {n} (x y : iN n) : iN 1 := pBind₂ x y icmpNe?
 
 @[simp_iN]
 def icmpUgt? {n} (x y : BitVec n) : iN 1 := bitvec (if x > y then 1 else 0)
 
-@[simp_iN, inst "icmp.ugt"]
+@[simp_iN]
 def icmpUgt {n} (x y : iN n) : iN 1 := pBind₂ x y icmpUgt?
 
 @[simp_iN]
 def icmpUge? {n} (x y : BitVec n) : iN 1 := bitvec (if x >= y then 1 else 0)
 
-@[simp_iN, inst "icmp.uge"]
+@[simp_iN]
 def icmpUge {n} (x y : iN n) : iN 1 := pBind₂ x y icmpUge?
 
 @[simp_iN]
 def icmpUlt? {n} (x y : BitVec n) : iN 1 := bitvec (if x < y then 1 else 0)
 
-@[simp_iN, inst "icmp.ult"]
+@[simp_iN]
 def icmpUlt {n} (x y : iN n) : iN 1 := pBind₂ x y icmpUlt?
 
 @[simp_iN]
 def icmpUle? {n} (x y : BitVec n) : iN 1 := bitvec (if x <= y then 1 else 0)
 
-@[simp_iN, inst "icmp.ule"]
+@[simp_iN]
 def icmpUle {n} (x y : iN n) : iN 1 := pBind₂ x y icmpUle?
 
 @[simp_iN]
 def icmpSgt? {n} (x y : BitVec n) : iN 1 := bitvec (if x.sle y then 0 else 1) -- inverse
 
-@[simp_iN, inst "icmp.sgt"]
+@[simp_iN]
 def icmpSgt {n} (x y : iN n) : iN 1 := pBind₂ x y icmpSgt?
 
 @[simp_iN]
 def icmpSge? {n} (x y : BitVec n) : iN 1 := bitvec (if x.slt y then 0 else 1) -- inverse
 
-@[simp_iN, inst "icmp.sge"]
+@[simp_iN]
 def icmpSge {n} (x y : iN n) : iN 1 := pBind₂ x y icmpSge?
 
 @[simp_iN]
 def icmpSlt? {n} (x y : BitVec n) : iN 1 := bitvec (if x.slt y then 1 else 0)
 
-@[simp_iN, inst "icmp.slt"]
+@[simp_iN]
 def icmpSlt {n} (x y : iN n) : iN 1 := pBind₂ x y icmpSlt?
 
 @[simp_iN]
 def icmpSle? {n} (x y : BitVec n) : iN 1 := bitvec (if x.sle y then 1 else 0)
 
-@[simp_iN, inst "icmp.sle"]
+@[simp_iN]
 def icmpSle {n} (x y : iN n) : iN 1 := pBind₂ x y icmpSle?
 
 infixl:55 " ==ᵤ " => iN.icmpEq
@@ -165,16 +164,16 @@ infixl:55 " ≤ₛ "  => iN.icmpSle
 infixl:55 " >ₛ "  => iN.icmpSgt
 infixl:55 " ≥ₛ "  => iN.icmpSge
 
-@[simp_iN, inst "and"]
+@[simp_iN]
 def and {n} (x y : iN n) : iN n := pBind₂ x y (fun a b => bitvec (a &&& b))
 
-@[simp_iN, inst "or"]
+@[simp_iN]
 def or {n} (x y : iN n) : iN n := pBind₂ x y (fun a b => bitvec (a ||| b))
 
-@[simp_iN, inst "not"]
+@[simp_iN]
 def not {n} (x : iN n) : iN n := pBind x (fun a => bitvec (~~~a))
 
-@[simp_iN, inst "xor"]
+@[simp_iN]
 def xor {n} (x y : iN n) : iN n := pBind₂ x y (fun a b => bitvec (a ^^^ b))
 
 instance : HAnd (iN n) (iN n) (iN n) where
@@ -198,7 +197,7 @@ def shl? {n} (a b : BitVec n) : iN n :=
   else
     bitvec (a <<< b)
 
-@[simp_iN, inst "shl"]
+@[simp_iN]
 def shl {n} (x y : iN n) : iN n := pBind₂ x y shl?
 
 @[simp_iN]
@@ -210,7 +209,7 @@ def shlNsw? {n} (a b : BitVec n) : iN n :=
   else
     shl? a b
 
-@[simp_iN, inst "shl.nsw"]
+@[simp_iN]
 def shlNsw {n} (x y : iN n) : iN n := pBind₂ x y shlNsw?
 
 @[simp_iN]
@@ -222,7 +221,7 @@ def shlNuw? {n} (a b : BitVec n) : iN n :=
   else
     shl? a b
 
-@[simp_iN, inst "shl.nuw"]
+@[simp_iN]
 def shlNuw {n} (x y : iN n) : iN n := pBind₂ x y shlNuw?
 
 instance : HShiftLeft (iN n) (iN n) (iN n) where
@@ -240,7 +239,7 @@ def lshr? {n} (a b : BitVec n) : iN n :=
   else
     bitvec (a >>> b)
 
-@[simp_iN, inst "lshr"]
+@[simp_iN]
 def lshr {n} (x y : iN n) : iN n := pBind₂ x y lshr?
 
 @[simp_iN]
@@ -254,7 +253,7 @@ def lshrExact? {n} (a b : BitVec n) : iN n :=
   else
     lshr? a b
 
-@[simp_iN, inst "lshr.exact"]
+@[simp_iN]
 def lshrExact {n} (x y : iN n) : iN n := pBind₂ x y lshrExact?
 
 infixl:75 " >>>ᵤ " => iN.lshr
@@ -269,7 +268,7 @@ def ashr? {n} (a b : BitVec n) : iN n :=
   else
     bitvec (a.sshiftRight' b)
 
-@[simp_iN, inst "ashr"]
+@[simp_iN]
 def ashr {n} (x y : iN n) : iN n := pBind₂ x y ashr?
 
 @[simp_iN]
@@ -283,11 +282,25 @@ def ashrExact? {n} (a b : BitVec n) : iN n :=
   else
     ashr? a b
 
-@[simp_iN, inst "ashr.exact"]
+@[simp_iN]
 def ashrExact {n} (x y : iN n) : iN n := pBind₂ x y ashrExact?
 
 infixl:75 " >>>ₛ " => iN.ashr
 infixl:75 " >>>ₛexact " => iN.ashrExact
+
+@[simp_iN]
+def sdiv? {n} (a b : BitVec n) : iN n :=
+  if b == 0 then
+    poison
+  else if b == -1 && a == BitVec.intMin n then
+    poison
+  else
+    bitvec (a.sdiv b)
+
+@[simp_iN]
+def sdiv {n} (x y : iN n) : iN n := pBind₂ x y sdiv?
+
+infixl:70 " /ₛ " => iN.sdiv
 
 end iN
 
@@ -322,4 +335,5 @@ section norm_eqs_simp_iN
 @[simp_iN] theorem bitvec_lshrExact_eq (x y : iN n) : x >>>ᵤexact y = iN.lshrExact x y := rfl
 @[simp_iN] theorem bitvec_ashr_eq (x y : iN n) : x >>>ₛ y = iN.ashr x y := rfl
 @[simp_iN] theorem bitvec_ashrExact_eq (x y : iN n) : x >>>ₛexact y = iN.ashrExact x y := rfl
+@[simp_iN] theorem bitvec_sdiv_eq (x y : iN n) : x /ₛ y = iN.sdiv x y := rfl
 end norm_eqs_simp_iN
