programs/mean_s32/eclass.lean
@@ -1,0 +1,33 @@
+import theorems.iN
+
+import Lean
+open Lean Parser Elab Meta Tactic
+
+def root₁ (x y : iN 32) := (x +nsw y) >>>ₛ 1
+def root₂ (x y : iN 32) := (x +nsw y) /ₛ 2
+
+#eval (root₁ 100 50)
+#eval (root₂ 100 50)
+
+theorem comm (x y : iN 32) : x +nsw y ~> y +nsw x := by
+  cases x
+  cases y
+  all_goals simp [simp_iN]
+  bv_decide
+
+theorem rewrite_test₁ (x y : iN 32) : x +nsw y + 1 ~> y +nsw x + 1 := by
+  exact Rewrite.congrApp (fun x => x + 1) (by simp [simp_iN]) (comm x y)
+
+theorem rewrite_test₂ (x y : iN 32) : x +nsw y + 1 ~> y +nsw x + 1 := by
+  apply_rw comm
+
+/-
+partial def elabRoot : Syntax → MetaM Expr
+ -/
+elab "⟨⟨" func:term "⟩⟩" : term => do
+  let func ← Term.elabTerm func none
+
+  dbg_trace func
+  return func
+
+def root := ⟨⟨root₁⟩⟩
