theorems/iN.lean
@@ -1,7 +1,8 @@
 import theorems.iN.SimpSets
 import theorems.iN.iN_def
 import theorems.iN.iN_llvm
-import theorems.iN.iN_tactics
 import theorems.iN.iN_lemmas
 import theorems.iN.iN_rewrite
-import theorems.Core.Attrs.Attrs
+import theorems.iN.iN_tactic_blast
+import theorems.iN.iN_tactic_rewrite
+--import theorems.Core.Attrs.Attrs
