theorems/iN/iN_tactic_rewrite.lean
@@ -1,0 +1,86 @@
+import Lean
+import theorems.iN.iN_def
+import theorems.iN.iN_rewrite
+
+open Lean Elab Tactic Meta
+
+/-- On a goal of `lhs ~> rhs`, apply a rewrite of the form `x ~> y`.  -/
+elab "apply_rewrite" t:term : tactic => withMainContext do
+  let mvarId ← getMainGoal
+
+  let matchRewrite (e : Expr) : MetaM (Expr × Expr × Expr) := do
+    match_expr e with
+    | Rewrite n lhs rhs => return (n, lhs, rhs)
+    | _ => throwTacticEx `apply_rewrite mvarId m!"not a rewrite{indentExpr e}"
+
+  let heq ← elabTerm t none true
+
+  --let heqIn := heq
+  let heqType ← instantiateMVars (← inferType heq)
+  let (newMVars, _, heqType) ← forallMetaTelescopeReducing heqType
+  /- `∀ (x y : iN 32), expr` into `expr`. -/
+  let heq := mkAppN heq newMVars
+
+  let occs : Occurrences := .all
+  let e ← getMainTarget
+  let e ← instantiateMVars e
+
+  let (n, lhs, rhs) ← matchRewrite e
+  let (_, x, y) ← matchRewrite heqType
+
+  -- h: x ~> y
+  -- ⊢ lhs ~> rhs
+  let lhsAbst ← kabstract lhs x occs
+  unless lhsAbst.hasLooseBVars do
+    throwTacticEx `apply_rewrite mvarId m!"did not find instance of the pattern in the target expression{indentExpr lhs}"
+
+  let α := (Expr.app (.const `iN []) n)
+  let motive := Lean.mkLambda `_a BinderInfo.default α lhsAbst
+
+  try
+    check motive
+  catch ex =>
+    throwTacticEx `apply_rewrite mvarId m!"motive is not type correct:{indentD motive}\nError: {ex.toMessageData}"
+
+  /- Proves `f poison = poison`. -/
+  let proveCongruence (motive : Expr) : MetaM Expr := do
+    let poison := mkApp (.const ``poison []) n
+    let poison_app := mkApp motive poison
+    let goalType ← mkEq poison_app poison
+
+    let proofMVar ← mkFreshExprMVar goalType .synthetic `h_cong_proof
+
+    let ctx ← Simp.mkContext
+      (config := { beta := true })
+      (simpTheorems := #[← getSimpTheorems, ← iNInst.getTheorems])
+      (congrTheorems := (← getSimpCongrTheorems))
+    let (result?, _) ← simpGoal proofMVar.mvarId! ctx
+
+    if let some (_, x) := result? then
+      throwTacticEx `apply_rewrite x
+        m!"unable to prove congruence goal `motive poison = poison` automatically with `simp [simp_iN]`"
+
+    instantiateMVars proofMVar
+
+  let motiveProof ← proveCongruence motive
+  let congrProof ← mkAppM ``Rewrite.congrApp #[motive, motiveProof, heq]
+
+  /- Construct final proof term with `Rewrite.trans` and a new goal. -/
+  let unreducedLhsNew := mkApp motive y
+  let newGoalType := mkAppN (.const ``Rewrite []) #[n, unreducedLhsNew, rhs]
+  let newGoalMVar ← mkFreshExprMVar (some newGoalType)
+  let fullProof ← mkAppM ``Rewrite.trans #[congrProof, newGoalMVar]
+  mvarId.assign fullProof
+
+  let newGoalId := newGoalMVar.mvarId!
+  let (n_new, unreducedLhs, rhs_new) ← matchRewrite (← newGoalId.getType)
+
+  /- Beta reduce the annoying motive. -/
+  let reducedLhs ← Core.betaReduce unreducedLhs
+  let finalGoalType := mkAppN (.const ``Rewrite []) #[n_new, reducedLhs, rhs_new]
+  let finalGoalId ← newGoalId.change finalGoalType
+
+  replaceMainGoal [finalGoalId]
+
+macro "apply_rw " t:term : tactic =>
+  `(tactic| (apply_rewrite $t; try (with_reducible rfl)))
